Factor out repeated parts of HavocPrecondition into separate predicate

src/backend/dafny/Indistinguishable.dfy
@@ -40,6 +40,16 @@ predicate {:induction false} ImmutablesUnchanged(objs: ObjList, objs': ObjList) 
           AssocGet(AssocGet(objs, k).val.locals, l).val == AssocGet(AssocGet(objs', k).val.locals, l).val
 }
 
+predicate {:induction false} HavocedList(objs: ObjList, objs1: ObjList)
+{
+    EqualKeys(objs, objs1) &&
+    (forall k: Addr ::
+        AssocGet(objs, k).Some? && AssocGet(objs1, k).Some? ==>
+        AssocGet(objs, k).val.immutables == AssocGet(objs1, k).val.immutables) &&
+    ImmutablesUnchanged(objs, objs1) &&
+    (forall k: Addr :: AssocGet(objs, k).Some? && AssocGet(objs1, k).Some? ==> EqualKeys(AssocGet(objs, k).val.locals, AssocGet(objs1, k).val.locals))
+}
+
 predicate {:induction false} HavocPrecondition(
     ctx1: Context, ctx2: Context, 
     addr1: Value, addr2: Value, 
@@ -52,18 +62,8 @@ predicate {:induction false} HavocPrecondition(
     Inv(ctx1, ctx2, addr1.addr, addr2.addr) &&
     var ctx1' := ctx1.(objs := objs1);
     var ctx2' := ctx2.(objs := objs2);
-    EqualKeys(ctx1.objs, objs1) &&
-    EqualKeys(ctx2.objs, objs2) &&
-    (forall k: Addr ::
-        AssocGet(ctx1.objs, k).Some? && AssocGet(objs1, k).Some? ==>
-        AssocGet(ctx1.objs, k).val.immutables == AssocGet(objs1, k).val.immutables) &&
-    (forall k: Addr ::
-        AssocGet(ctx2.objs, k).Some? && AssocGet(objs2, k).Some? ==>
-        AssocGet(ctx2.objs, k).val.immutables == AssocGet(objs2, k).val.immutables) &&
-    ImmutablesUnchanged(ctx1.objs, objs1) &&
-    ImmutablesUnchanged(ctx2.objs, objs2) &&
-    (forall k: Addr :: AssocGet(ctx1.objs, k).Some? && AssocGet(objs1, k).Some? ==> EqualKeys(AssocGet(ctx1.objs, k).val.locals, AssocGet(objs1, k).val.locals)) &&
-    (forall k: Addr :: AssocGet(ctx2.objs, k).Some? && AssocGet(objs2, k).Some? ==> EqualKeys(AssocGet(ctx2.objs, k).val.locals, AssocGet(objs2, k).val.locals)) &&
+    HavocedList(ctx1.objs, objs1) &&
+    HavocedList(ctx2.objs, objs2) &&
     (forall k, l :: AssocGet(objs1, k).Some? && AssocGet(AssocGet(objs1, k).val.locals, l).Some? ==> AssocGet(AssocGet(objs1, k).val.locals, l).val != Nil && (AssocGet(AssocGet(objs1, k).val.locals, l).val.Ref? ==> AssocGet(AssocGet(objs1, k).val.locals, l).val.addr < addr1.addr)) &&
     (forall k, l :: AssocGet(objs2, k).Some? && AssocGet(AssocGet(objs2, k).val.locals, l).Some? ==> AssocGet(AssocGet(objs2, k).val.locals, l).val != Nil && (AssocGet(AssocGet(objs2, k).val.locals, l).val.Ref? ==> AssocGet(AssocGet(objs2, k).val.locals, l).val.addr < addr2.addr)) &&
     Inv(ctx1', ctx2', addr1.addr, addr2.addr)
